Add definitions and support for 32b arithmetic ins.

otbn_model/spec/types.dfy
@@ -24,4 +24,37 @@ type uint128 = i:int | 0 <= i < 0x1_00000000_00000000_00000000_00000000
 	
 datatype Bignum = Bignum(l7:uint32, l6:uint32, l5:uint32, l4:uint32, l3:uint32, l2:uint32, l1:uint32, l0:uint32)
 
+/////////////////
+// BitsOfByte
+/////////////////
+
+newtype twobits = i:int | 0 <= i < 4
+datatype BitsOfByte = BitsOfByte(lo:twobits,
+                                 mid_lo:twobits,
+                                 mid_hi:twobits,
+                                 hi:twobits)
+
+function bits_to_byte(bits:BitsOfByte) : uint8
+{
+    64 * (bits.hi as uint8) + 16 * (bits.mid_hi as uint8) + 4 * (bits.mid_lo as uint8) + (bits.lo as uint8)
+}
+
+function byte_to_bits(b:uint8) : BitsOfByte
+{
+    BitsOfByte((b % 4) as twobits, ((b / 4) % 4) as twobits, ((b / 16) % 4) as twobits, ((b / 64) % 4) as twobits)
+}
+
+/////////////////
+// Bit vectors
+/////////////////
+
+function method {:opaque} BitsToWord(b:bv32) : uint32 { b as uint32 }
+function method {:opaque} WordToBits(w:uint32) : bv32 { w as bv32 }
+
+lemma {:axiom} lemma_BitsToWordToBits(b:bv32)
+    ensures WordToBits(BitsToWord(b)) == b;
+
+lemma {:axiom} lemma_WordToBitsToWord(w:uint32)
+    ensures BitsToWord(WordToBits(w)) == w;
+
 } // end module types
